演習3.5.16は後回し！！

practice/TaPL/coq/arith/chap3.v
@@ -341,8 +341,8 @@ End ArithNat.
 Module ArithNatBad.
 
 Inductive t: Type :=
-| true
-| false
+| tru
+| fls
 | If (t1 t2 t3: t)
 | O
 | succ (t1: t)
@@ -356,13 +356,13 @@ Inductive NatValue: t -> Prop :=
 | nv_S : forall nv1, NatValue nv1 -> NatValue (succ nv1).
 
 Inductive value: t -> Prop :=
-| v_tru : value true
-| v_fls : value false
+| v_tru : value tru
+| v_fls : value fls
 | v_nat : forall t1, NatValue t1 -> value t1.
 
 Inductive BadNat : t -> Prop :=
-| bn_true : BadNat true
-| bn_false : BadNat false
+| bn_tru : BadNat tru
+| bn_fls : BadNat fls
 | bn_wrong : BadNat wrong.
 
 Inductive BadBool : t -> Prop :=
@@ -370,39 +370,408 @@ Inductive BadBool : t -> Prop :=
 | bb_wrong : BadBool wrong.
 
 Reserved Notation " t '-->' t' " (at level 40).
-Inductive step: t -> t -> Prop :=
-| E_IfTrue : forall t2 t3,
-    If true t2 t3 --> t2
-| E_IfFalse : forall t2 t3,
-    If false t2 t3 --> t3
-| E_If : forall t1 t1' t2 t3,
+Inductive estep: t -> t -> Prop :=
+| Ee_IfTrue : forall t2 t3,
+    If tru t2 t3 --> t2
+| Ee_IfFalse : forall t2 t3,
+    If fls t2 t3 --> t3
+| Ee_If : forall t1 t1' t2 t3,
     t1 --> t1' ->
     If t1 t2 t3 --> If t1' t2 t3
-| E_Succ : forall t1 t1',
+| Ee_Succ : forall t1 t1',
     t1 --> t1' -> succ t1 --> succ t1'
-| E_PredZero :
+| Ee_PredZero :
     pred O --> O
-| E_PredSucc : forall nv1,
+| Ee_PredSucc : forall nv1,
     NatValue nv1 -> pred (succ nv1) --> nv1
-| E_Pred : forall t1 t1',
-    t1 --> t1' -> pred t1 --> t1'
-| E_IsZeroZero :
-    iszero O --> true
-| E_IsZeroSucc : forall nv1,
-    NatValue nv1 -> iszero (succ nv1) --> false
-| E_IsZero : forall t1 t1',
+| Ee_Pred : forall t1 t1',
+    t1 --> t1' -> pred t1 --> pred t1'
+| Ee_IsZeroZero :
+    iszero O --> tru
+| Ee_IsZeroSucc : forall nv1,
+    NatValue nv1 -> iszero (succ nv1) --> fls
+| Ee_IsZero : forall t1 t1',
     t1 --> t1' -> iszero t1 --> iszero t1'
 
 (*行き詰まり処理*)
-| E_IfWrong : forall t1 t2 t3,
+| Ee_IfWrong : forall t1 t2 t3,
     BadBool t1 -> If t1 t2 t3 --> wrong
 | E_SuccWrong : forall t1,
     BadNat t1 -> succ t1 --> wrong
-| E_PredWrong : forall t1,
+| Ee_PredWrong : forall t1,
     BadNat t1 -> pred t1 --> wrong
-| E_IsZeroWrong : forall t1,
+| Ee_IsZeroWrong : forall t1,
     BadNat t1 -> iszero t1 --> wrong
 
-  where " t '-->' t' " := (step t t').
+  where " t '-->' t' " := (estep t t').
+
+Reserved Notation " t '-->o' t' " (at level 40).
+Inductive step: t -> t -> Prop :=
+| E_IfTrue : forall t2 t3,
+    If tru t2 t3 -->o t2
+| E_IfFalse : forall t2 t3,
+    If fls t2 t3 -->o t3
+| E_If : forall t1 t1' t2 t3,
+    t1 -->o t1' ->
+    If t1 t2 t3 -->o If t1' t2 t3
+| E_Succ : forall t1 t1',
+    t1 -->o t1' -> succ t1 -->o succ t1'
+| E_PredZero :
+    pred O -->o O
+| E_PredSucc : forall nv1,
+    NatValue nv1 -> pred (succ nv1) -->o nv1
+| E_Pred : forall t1 t1',
+    t1 -->o t1' -> pred t1 -->o pred t1'
+| E_IsZeroZero :
+    iszero O -->o tru
+| E_IsZeroSucc : forall nv1,
+    NatValue nv1 -> iszero (succ nv1) -->o fls
+| E_IsZero : forall t1 t1',
+    t1 -->o t1' -> iszero t1 -->o iszero t1'
+
+  where " t '-->o' t' " := (step t t').
+
+Definition stop (t1: t) :=
+  not (value t1) /\ not (exists t1', t1 -->o t1').
+
+Lemma existstop:
+  exists t1, stop t1.
+Proof.
+  exists (iszero tru).
+  split.
+  intro H; inversion H. inversion H0.
+  intro H. inversion H. inversion H0. inversion H2.
+Qed.
+
+
+Ltac solve_by_inverts n :=
+  match goal with | H : ?T |- _ =>
+  match type of T with Prop =>
+    solve [
+      inversion H;
+      match n with S (S (?n')) => subst; solve_by_inverts (S n') end ]
+  end end.
+
+Ltac solve_by_invert :=
+  solve_by_inverts 1.
+
+Fixpoint Good (t1: t) : bool :=
+  match t1 with
+  | wrong => false
+  | If t1' t2 t3 => andb (Good t1') (andb (Good t2) (Good t3))
+  | succ t1' => Good t1'
+  | pred t1' => Good t1'
+  | iszero t1' => Good t1'
+  | _ => true
+  end.
+
+Lemma nv_notstep : forall nv1,
+    NatValue nv1 -> not (exists t1, nv1 --> t1).
+Proof.
+  intros. induction H; intro H1.
+  inversion H1. inversion H.
+  inversion H1. inversion H0; subst.
+  induction IHNatValue.
+  exists t1'; assumption.
+  inversion H3; subst; solve_by_invert.
+Qed.
+
+Lemma NatValuesucc: forall nv,
+    NatValue nv -> not (exists t1', succ nv --> t1').
+Proof.
+  intros. induction H.
+  intro H. inversion H. inversion H0; try solve_by_invert.
+  intro HH. inversion HH. inversion H0; subst.
+  induction IHNatValue. exists t1'; auto.
+  inversion H2.
+Qed.
+
+Lemma A3: forall t1 t1' t1'',
+     t1 --> t1' -> t1 --> t1'' -> t1' = t1''.
+Proof.
+  intros. generalize dependent t1''; induction H; intros.
+  -
+    inversion H0; subst; auto; try solve_by_invert. inversion H4. inversion H.
+  -
+    inversion H0; subst; auto; try solve_by_inverts 2.
+  -
+    inversion H0; subst; try solve_by_invert.
+    apply IHestep in H5; subst; auto.
+    inversion H5; subst. induction (nv_notstep t1); auto. exists t1'; auto.
+    inversion H.
+  -
+    inversion H0; subst. rewrite IHestep with (t1'':=t1'0); auto.
+    inversion H2; subst; try solve_by_invert.
+  -
+    inversion H0; auto; try solve_by_invert.
+  -
+    inversion H0; subst; auto.
+    induction (NatValuesucc nv1); auto. exists t1'; auto.
+    inversion H2.
+  -
+    inversion H0;subst. inversion H.
+    induction (NatValuesucc t1''); auto. exists t1'; auto. 
+    apply IHestep in H2; subst; auto.
+    inversion H2; subst; try solve_by_invert.
+  -
+    inversion H0; auto; try solve_by_invert.
+  -
+    inversion H0; subst; auto.
+    induction (NatValuesucc nv1); auto. exists t1'; auto.
+    inversion H2.
+  -
+    inversion H0; subst; auto; try solve_by_invert.
+    induction (NatValuesucc nv1); auto. exists t1'; auto.
+    apply IHestep in H2; subst; auto.
+    inversion H2; subst; try solve_by_invert.
+  -
+    inversion H0; subst; try solve_by_inverts 2; auto.
+    inversion H; subst; try solve_by_invert.
+    induction (nv_notstep t1); auto. exists t1'; auto.
+  -
+    inversion H; subst.
+    inversion H0; subst; try solve_by_invert; auto.
+    inversion H0; subst; try solve_by_invert; auto.
+    inversion H0; subst; auto. inversion H2.
+  -
+    inversion H0; subst; try solve_by_invert; auto.
+    inversion H; subst; try solve_by_invert.
+  -
+    inversion H0; subst; try solve_by_invert; auto.
+    inversion H; subst; try solve_by_invert.
+Qed.
+
+
+Lemma IfStopWrong: forall t1 t2 t3,
+    stop (If t1 t2 t3) -> not (exists t1', t1 -->o t1').
+Proof.
+  intros.
+  induction t1.
+  - (*tur*)
+    inversion H. induction H1. exists t2; apply E_IfTrue.
+  - (*fls*)
+    inversion H. induction H1; exists t3; apply E_IfFalse.
+  - (*If*)
+    intros HH.
+    inversion HH.
+    inversion H.
+    inversion H0; subst;
+    induction H2; eexists; eapply E_If; apply H0.
+  -
+    intro HH; inversion HH. inversion H0.
+  -
+    intro HH; inversion HH. inversion H0.
+    inversion H. induction H5.
+    eexists. eapply E_If. eapply E_Succ. apply H2.
+  -
+    intros HH; inversion HH. inversion H. inversion H0; subst;
+    induction H2; subst; eexists; eapply E_If; eassumption.
+  -
+    intros HH; inversion HH; inversion H. inversion H0; subst;
+    induction H2; eexists; eapply E_If; eassumption.
+  -
+    intros HH; inversion HH; inversion H. inversion H0; subst;
+    induction H2; eexists; eapply E_If; eassumption.
+Qed.
+
+Notation multiestep := (multi estep).
+Notation "t1 '-->*' t2" := (multiestep t1 t2) (at level 40).
+
+Notation multistep := (multi step).
+Notation "t1 '-->o*' t2" := (multistep t1 t2) (at level 40).
+
+
+Lemma Iftrans : forall t1 t2 t3 t1',
+    t1 -->* t1' -> If t1 t2 t3 -->* If t1' t2 t3.
+Proof.
+  intros. induction H.
+  apply multi_refl. eapply multi_step. apply Ee_If. eassumption.
+  assumption.
+Qed.
+
+
+Lemma multitrans: forall t1 t2 t3,
+    t1 -->* t2 -> t2 -->* t3 -> t1 -->* t3.
+Proof.
+  intros. generalize dependent t3. induction H; intros.
+  assumption.
+  eapply multi_step. apply H. apply IHmulti. assumption.
+Qed.
+
+
+Fixpoint NVBool (t1: t) : bool :=
+  match t1 with
+  | O => true
+  | succ t1' => NVBool t1'
+  | _ => false
+  end.
+
+Lemma NVB_nv : forall t1,
+    NVBool t1 = true <-> NatValue t1.
+Proof.
+  split; intros.
+  -
+    induction t1; try solve_by_invert.
+    apply nv_O. apply nv_S. apply IHt1. inversion H; auto.
+  -
+    induction H; subst; auto.
+Qed.
+
+Lemma stepe : forall t1 t1',
+    t1 -->o t1' -> t1 --> t1'.
+Proof.
+  intros. induction H.
+  -
+    apply Ee_IfTrue.
+  -
+    apply Ee_IfFalse.
+  -
+    apply Ee_If; auto.
+  -
+    apply Ee_Succ; auto.
+  -
+    apply Ee_PredZero.
+  -
+    apply Ee_PredSucc; auto.
+  -
+    apply Ee_Pred; auto.
+  -
+    apply Ee_IsZeroZero.
+  -
+    apply Ee_IsZeroSucc; auto.
+  -
+    apply Ee_IsZero; auto.
+Qed.
+
+Lemma A4If : forall t1 t2 t3,
+    (Good (If t1 t2 t3)) = true -> stop (If t1 t2 t3) -> (If t1 t2 t3) -->* wrong.
+Proof.
+  intros. generalize dependent t3. generalize dependent t2. generalize dependent t1.
+  induction t1; intros.
+  -
+    inversion H0. induction H2. exists t2; apply E_IfTrue.
+  -
+    inversion H0. induction H2. exists t3; apply E_IfFalse.
+  -
+    destruct (Good (If t1_1 t1_2 t1_3)) eqn:IHH.
+
+    assert (stop (If t1_1 t1_2 t1_3)).
+    split; intro HH. inversion HH. inversion H1.
+    inversion HH. inversion H0. apply H3. exists (If x t2 t3). apply E_If; auto.
+
+    apply IHt1_1 in H1; auto.
+    apply Iftrans with (t2:= t2) (t3:= t3) in H1.
+
+    assert (If wrong t2 t3 -->* wrong).
+    eapply multi_step. apply Ee_IfWrong. apply bb_wrong.
+    apply multi_refl.
+    apply multitrans with (t3:= wrong) in H1; auto.
+
+    inversion H. apply andb_prop in H2. inversion H2. inversion H1. apply andb_prop in H5.
+    inversion H5. apply andb_prop in H6. inversion H6;  inversion IHH; subst.
+    rewrite H4 in H10. rewrite H7 in H10. rewrite H8 in H10. inversion H10.
+  -
+    eapply multi_step. apply Ee_IfWrong. apply bb_nat. apply nv_O. apply multi_refl.
+  -
+    generalize H0; intro H1.
+    apply IfStopWrong in H0.
+    destruct (Good (If t1 t2 t3)) eqn:IHH.
+    apply IHt1 in IHH.
+    inversion IHH; subst.
+
+    inversion H2; subst.
+    eapply multi_step. apply Ee_If. apply E_SuccWrong. apply bn_tru.
+    eapply multi_step. apply Ee_IfWrong. apply bb_wrong. apply multi_refl.
+
+    eapply multi_step. apply Ee_If. apply E_SuccWrong. apply bn_fls.
+    eapply multi_step. apply Ee_IfWrong. apply bb_wrong. apply multi_refl.
+
+    induction H0. exists (succ t1'). apply E_Succ; auto. admit.
+
+    inversion H8; subst.
+    eapply multi_step. apply Ee_IfWrong. apply bb_nat; apply nv_S; auto. apply multi_refl.
+    eapply multi_step. apply Ee_If; apply E_SuccWrong. apply bn_wrong. eapply multi_step. apply Ee_IfWrong.
+    apply bb_wrong. apply multi_refl.
+
+    split; intro HH; inversion HH; try solve_by_invert.
+    inversion H1. admit.
+
+    admit.
+  -
+Abort.
+
+
+
+Lemma A4: forall t1,
+    (Good t1) = true -> stop t1 -> t1 --> wrong.
+Proof.
+  induction t1; intros.
+  -
+    admit.
+  -
+    admit.
+  -
+    admit.
+  -
+Abort.
+
+
+Lemma NVstep: forall nv,
+    NatValue nv -> not (exists t1', succ nv -->o t1').
+Proof.
+  intros. induction H.
+  intro H. inversion H. inversion H0; try solve_by_invert.
+  intro HH. inversion HH. inversion H0; subst.
+  induction IHNatValue. exists t1'; auto.
+Qed.
+
+Lemma A5: forall t1 t2,
+    Good t1 = true -> Good t2 = false ->
+    t1 --> t2 -> stop t1.
+Proof.
+  intros. induction H1; try solve_by_invert.
+  -
+    try (inversion H; apply andb_prop in H2; inversion H2; rewrite H1 in H0; discriminate H0).
+  -
+    inversion H. apply andb_prop in H2. inversion H2. rewrite H3 in H0; discriminate.
+  -
+    split; intros HH. inversion HH. inversion H2.
+    inversion H0. inversion H. apply andb_prop in H4. inversion H4. rewrite H5 in H3.
+    destruct (Good t1') eqn:IHH. discriminate.
+    inversion HH. inversion H6; subst; try solve_by_invert.
+    destruct IHestep; auto. induction H8. exists t1'0; auto.
+  -
+    split; intro HH. inversion HH; subst. inversion H2; induction (nv_notstep t1); auto. exists t1'; auto.
+    inversion HH. inversion H2; subst. destruct IHestep; auto. induction H5. exists t1'0; auto.
+  -
+    inversion H. rewrite H3 in H0. inversion H0. 
+  -
+    inversion H. destruct IHestep; auto.
+    split; intro HH. inversion HH. inversion H5.
+    inversion HH. inversion H5; subst; try solve_by_invert.
+    induction H2. apply v_nat; apply nv_S; auto.
+    induction H4. exists t1'0; auto.
+  -
+    inversion H; inversion H0. destruct IHestep; auto.
+    split; intro HH. inversion HH. inversion H6.
+    inversion HH. inversion H6; subst; try solve_by_invert.
+    induction H2. apply v_nat; apply nv_S; auto.
+    induction H5. exists t1'0; auto.
+  -
+    inversion H1; subst; try solve_by_inverts 2.
+    split; intro HH; inversion HH. inversion H3.
+    inversion H3; subst; try solve_by_invert.
+    induction (NVstep t1); auto. exists (succ t1'). apply E_Succ; auto.
+  -
+    inversion H1; subst; try solve_by_invert;
+    split; intro HH;
+      inversion HH; inversion H2; subst; try solve_by_invert.
+  -
+    inversion H1; subst; try solve_by_invert;
+      split; intro HH; inversion HH;  try solve_by_inverts 2.
+  -
+    inversion H1; subst; try solve_by_invert;
+      split; intro HH; inversion HH;  try solve_by_inverts 2.
+Qed.
 
 End ArithNatBad.
